Rename Local PF things

src/ldrfpf/LocalPF.v
@@ -33,8 +33,8 @@ Set Implicit Arguments.
 
 
 
+Module PF.
 Section LOCALPF.
-  (** The Definition of the L-PF machine **)
   Variable L: Loc.t -> bool.
 
   Definition pf_event (e: ThreadEvent.t): Prop :=
@@ -48,82 +48,6 @@ Section LOCALPF.
       (<<CONSISTENT: Trace.consistent th tr_cert>>) /\
       (<<PFCERT: List.Forall (compose pf_event snd) tr_cert>>).
 
-  Inductive pf_step:
-    forall (e:ThreadEvent.t) (tid:Ident.t) (c1 c2:Configuration.t), Prop :=
-  | pf_step_intro
-      e tid c1 lang st1 lc1 e2 e3 st4 lc4 sc4 memory4
-      (TID: IdentMap.find tid c1.(Configuration.threads) = Some (existT _ lang st1, lc1))
-      (CANCELS: rtc (@Thread.cancel_step _) (Thread.mk _ st1 lc1 c1.(Configuration.sc) c1.(Configuration.memory)) e2)
-      (STEP: Thread.opt_step e e2 e3)
-      (RESERVES: rtc (@Thread.reserve_step _) e3 (Thread.mk _ st4 lc4 sc4 memory4))
-      (CONSISTENT: e <> ThreadEvent.failure -> pf_consistent (Thread.mk _ st4 lc4 sc4 memory4))
-      (PF: pf_event e)
-    :
-      pf_step e tid c1 (Configuration.mk (IdentMap.add tid (existT _ _ st4, lc4) c1.(Configuration.threads)) sc4 memory4)
-  .
-  Hint Constructors pf_step.
-
-  Inductive pf_machine_step: forall (e:MachineEvent.t) (tid:Ident.t) (c1 c2:Configuration.t), Prop :=
-  | pf_machine_step_intro
-      e tid c1 c2
-      (STEP: pf_step e tid c1 c2)
-    :
-      pf_machine_step (ThreadEvent.get_machine_event e) tid c1 c2
-  .
-  Hint Constructors pf_machine_step.
-
-  Inductive pf_all_step (c1 c2: Configuration.t): Prop :=
-  | pf_all_step_intro
-      e tid
-      (STEP: pf_step e tid c1 c2)
-  .
-  Hint Constructors pf_all_step.
-
-
-  (** The Definition of an L-PF race **)
-  Inductive reading_event (loc: Loc.t) (ts: Time.t):
-    forall (e: ThreadEvent.t), Prop :=
-  | reading_event_read
-      valr releasedr ordr
-    :
-      reading_event loc ts (ThreadEvent.read loc ts valr releasedr ordr)
-  | reading_event_update
-      to valr valw releasedr releasedw ordr ordw
-    :
-      reading_event loc ts (ThreadEvent.update loc ts to valr valw releasedr releasedw ordr ordw)
-  .
-
-  Inductive writing_event (loc: Loc.t) (ts: Time.t):
-    forall (e: ThreadEvent.t), Prop :=
-  | writing_event_write
-      from valw releasedw ordw
-      (ORD: Ordering.le ordw Ordering.relaxed)
-    :
-      writing_event loc ts (ThreadEvent.write loc from ts valw releasedw ordw)
-  | writing_event_update
-      from valr valw releasedr releasedw ordr ordw
-      (ORD: Ordering.le ordw Ordering.relaxed)
-    :
-      writing_event loc ts (ThreadEvent.update loc from ts valr valw releasedr releasedw ordr ordw)
-  .
-
-  Definition pf_racy_execution (c0: Configuration.t): Prop :=
-    forall tid0 c1 tid1 c2 c3
-           loc ts e0 e1
-           (LOC: L loc)
-           (TID: tid0 <> tid1)
-           (CSTEP0: pf_step e0 tid0 c0 c1)
-           (WRITE: writing_event loc ts e0)
-           (STEPS: rtc (pf_machine_step MachineEvent.silent tid1) c1 c2)
-           (CSTEP1: pf_step e1 tid1 c2 c3)
-           (READ: reading_event loc ts e1),
-      False.
-
-  Definition pf_racefree (c0: Configuration.t): Prop :=
-    forall c1
-           (CSTEPS: rtc pf_all_step c0 c1),
-      pf_racy_execution c1.
-
   Definition pf_promises (prom: Memory.t): Prop :=
     forall loc to from msg
            (LOC: L loc)
@@ -135,26 +59,6 @@ Section LOCALPF.
            (TID: IdentMap.find tid c.(Configuration.threads) = Some (existT _ lang st, lc)),
       pf_promises lc.(Local.promises).
 
-  Inductive pf_racy_state (c0: Configuration.t): Prop :=
-  | pf_race_intro
-      c1 c2
-      tid0 tid1 e0 e1
-      lang st0 lc0 th1 th2
-      tr pf loc ts
-      (STEPS: rtc (pf_machine_step MachineEvent.silent tid0) c0 c1)
-      (WRITE_STEP: pf_step e0 tid0 c1 c2)
-      (WRITE: writing_event loc ts e0)
-      (FIND: IdentMap.find tid1 c2.(Configuration.threads) = Some (existT _ lang st0, lc0))
-      (THREAD_STEPS: Trace.steps tr (Thread.mk _ st0 lc0 c2.(Configuration.sc) c2.(Configuration.memory)) th1)
-      (PF: List.Forall (compose pf_event snd) tr)
-      (CONS: Local.promise_consistent th1.(Thread.local))
-      (READ_STEP: Thread.step pf e1 th1 th2)
-      (READ: reading_event loc ts e1)
-      (LOC: L loc)
-  .
-
-
-  (** Properties of the L-PF machine **)
   Lemma pf_consistent_consistent lang (th: Thread.t lang)
         (CONSISTENT: pf_consistent th)
     :
@@ -165,99 +69,6 @@ Section LOCALPF.
     { eapply Trace.silent_steps_tau_steps in STEPS; eauto.
       left. unfold Thread.steps_failure. esplits; eauto. }
     { eapply Trace.silent_steps_tau_steps in STEPS; eauto. }
-  Qed.
-
-  Inductive opt_pf_machine_step:
-    forall (e: MachineEvent.t) (tid: Ident.t) (c1 c2: Configuration.t), Prop :=
-  | opt_pf_machine_step_none
-      tid c:
-      opt_pf_machine_step MachineEvent.silent tid c c
-  | opt_pf_machine_step_some
-      e tid c1 c2
-      (STEP: pf_machine_step e tid c1 c2):
-      opt_pf_machine_step e tid c1 c2
-  .
-  Hint Constructors opt_pf_machine_step.
-
-  Definition tau_pf_machine_step := union (pf_machine_step MachineEvent.silent).
-
-  Inductive pf_steps:
-    forall (es: list ThreadEvent.t) (tid: Ident.t) (c1 c2:Configuration.t), Prop :=
-  | pf_steps_nil
-      tid c1
-    :
-      pf_steps [] tid c1 c1
-  | pf_steps_cons
-      ehd etl tid c1 c2 c3
-      (STEP: pf_step ehd tid c1 c2)
-      (STEPS: pf_steps etl tid c2 c3)
-    :
-      pf_steps (ehd :: etl) tid c1 c3
-  .
-  Hint Constructors pf_steps.
-
-  Lemma pf_steps_rtc_pf_all_step es tid c1 c2
-        (STEPS: pf_steps es tid c1 c2)
-    :
-      rtc pf_all_step c1 c2.
-  Proof.
-    induction STEPS; eauto.
-  Qed.
-
-  Lemma pf_steps_split es0 es1 tid c0 c2
-        (STEPS: pf_steps (es0 ++ es1) tid c0 c2)
-    :
-      exists c1,
-        (<<STEPS0: pf_steps es0 tid c0 c1>>) /\
-        (<<STEPS1: pf_steps es1 tid c1 c2>>).
-  Proof.
-    ginduction es0; eauto. i. ss. inv STEPS.
-    exploit IHes0; eauto. i. des.
-    esplits; eauto.
-  Qed.
-
-  Lemma silent_pf_steps_tau_pf_machine_steps es tid c1 c2
-        (STEPS: pf_steps es tid c1 c2)
-        (SILENT: List.Forall (fun e => ThreadEvent.get_machine_event e = MachineEvent.silent) es)
-    :
-      rtc (pf_machine_step MachineEvent.silent tid) c1 c2.
-  Proof.
-    ginduction es; i.
-    { inv STEPS. eauto. }
-    { inv STEPS. inv SILENT. exploit IHes; eauto.
-      i. econs 2; eauto. rewrite <- H1. econs; eauto. }
-  Qed.
-
-  Lemma step_pf_racefree c0 c1 e tid
-        (RACEFREE: pf_racefree c0)
-        (STEP: pf_step e tid c0 c1)
-    :
-      pf_racefree c1.
-  Proof.
-    unfold pf_racefree in *. i.
-    eapply RACEFREE. econs 2; eauto.
-  Qed.
-
-  Lemma rtc_tau_machine_step_pf_racefree c0 c1
-        (RACEFREE: pf_racefree c0)
-        (STEP: rtc tau_pf_machine_step c0 c1)
-    :
-      pf_racefree c1.
-  Proof.
-    ginduction STEP; eauto.
-    i. eapply IHSTEP. inv H. inv USTEP.
-    eapply step_pf_racefree; eauto.
-  Qed.
-
-  Lemma steps_pf_racefree es tid c0 c1
-        (RACEFREE: pf_racefree c0)
-        (STEPS: pf_steps es tid c0 c1)
-    :
-      pf_racefree c1.
-  Proof.
-    ginduction STEPS; eauto.
-    i. eapply IHSTEPS.
-    eapply step_pf_racefree; eauto.
   Qed.
 
   Lemma pf_promises_promise prom0 mem0 loc from to msg prom1 mem1 kind
@@ -365,21 +176,7 @@ Section LOCALPF.
     erewrite Memory.bot_get in GET. ss.
   Qed.
 
-  Lemma pf_configuration_step tid c1 c2 e
-        (STEP: pf_step e tid c1 c2)
-        (PF: pf_configuration c1)
-    :
-      pf_configuration c2.
-  Proof.
-    inv STEP. unfold pf_configuration in *. i. ss.
-    erewrite IdentMap.gsspec in TID0. des_ifs; eauto.
-    dep_clarify. eapply PF in TID.
-    eapply pf_promises_cancel_steps in CANCELS; eauto.
-    eapply pf_promises_opt_step in STEP0; eauto.
-    eapply pf_promises_reserve_steps in RESERVES; eauto.
-  Qed.
-
-  Lemma pf_promises_pf_step_pf_event lang (th0 th1: Thread.t lang) e
+  Lemma pf_promises_step_event lang (th0 th1: Thread.t lang) e
         (STEP: Thread.step true e th0 th1)
         (PROMISES: pf_promises th0.(Thread.local).(Local.promises))
     :
@@ -391,7 +188,7 @@ Section LOCALPF.
     eapply PROMISES in GET; eauto. clarify.
   Qed.
 
-  Lemma pf_promises_pf_steps_pf_trace lang (th0 th1: Thread.t lang)
+  Lemma pf_promises_steps_trace lang (th0 th1: Thread.t lang)
         (STEPS: rtc (tau (Thread.step true)) th0 th1)
         (PROMISES: pf_promises th0.(Thread.local).(Local.promises))
     :
@@ -402,210 +199,10 @@ Section LOCALPF.
   Proof.
     ginduction STEPS; eauto; i.
     { exists []. splits; eauto. }
-    i. inv H. hexploit pf_promises_pf_step_pf_event; eauto. intros PF.
+    i. inv H. hexploit pf_promises_step_event; eauto. intros PF.
     hexploit pf_promises_step; eauto. intros PROMISES0.
     exploit IHSTEPS; eauto. i. des. esplits; eauto.
   Qed.
-
-  Lemma pf_promises_consistent_pf_consistent lang (th: Thread.t lang)
-        (CONSISTENT: Thread.consistent th)
-        (WF: Local.wf th.(Thread.local) th.(Thread.memory))
-        (MEM: Memory.closed th.(Thread.memory))
-        (PROMISES: pf_promises th.(Thread.local).(Local.promises))
-    :
-      pf_consistent th.
-  Proof.
-    eapply consistent_pf_consistent in CONSISTENT; eauto.
-    exploit Memory.cap_exists; eauto. i. des.
-    exploit Memory.max_concrete_timemap_exists.
-    { eapply Memory.cap_closed; eauto. } i. des.
-    exploit CONSISTENT; eauto. i. des.
-    { eapply pf_promises_pf_steps_pf_trace in STEPS; eauto. des.
-      exists tr. splits; auto. ii.
-      exploit (@Memory.cap_inj th.(Thread.memory) mem2 mem1); eauto. i. subst.
-      exploit (@Memory.max_concrete_timemap_inj mem1 tm sc1); eauto. i. subst.
-      esplits; eauto.
-    }
-    { eapply pf_promises_pf_steps_pf_trace in STEPS; eauto. des.
-      exists tr. splits; auto. ii.
-      exploit (@Memory.cap_inj th.(Thread.memory) mem2 mem1); eauto. i. subst.
-      exploit (@Memory.max_concrete_timemap_inj mem1 tm sc1); eauto. i. subst.
-      esplits; eauto.
-    }
-  Qed.
-
-  Lemma pf_event_configuration_step_pf_step c1 c2 e tid
-        (STEP: SConfiguration.step e tid c1 c2)
-        (WF: Configuration.wf c1)
-        (PF: pf_configuration c1)
-        (EVENT: pf_event e)
-    :
-      pf_step e tid c1 c2.
-  Proof.
-    inv STEP. econs; eauto. i.
-    exploit Thread.rtc_cancel_step_future; eauto; try eapply WF; eauto. ss. i. des.
-    exploit Thread.opt_step_future; eauto. ss. i. des.
-    exploit Thread.rtc_reserve_step_future; eauto; try eapply WF; eauto. ss. i. des.
-    hexploit pf_promises_cancel_steps; eauto. i. ss.
-    hexploit pf_promises_opt_step; eauto. i. ss.
-    hexploit pf_promises_reserve_steps; eauto. i. ss.
-    eapply pf_promises_consistent_pf_consistent; eauto.
-  Qed.
-
-  Lemma reservation_only_step_pf_step tid c1 c2
-        (STEP: SConfiguration.reservation_only_step tid c1 c2)
-        (WF: Configuration.wf c1)
-        (PF: pf_configuration c1)
-    :
-      pf_step ThreadEvent.silent tid c1 c2.
-  Proof.
-    eapply SConfiguration.reservation_only_step_step in STEP.
-    eapply pf_event_configuration_step_pf_step; eauto. ss.
-  Qed.
-
-  Lemma pf_step_pf_event_configuration_step c1 c2 e tid
-        (STEP: pf_step e tid c1 c2)
-        (WF: Configuration.wf c1)
-    :
-      (<<STEP: SConfiguration.step e tid c1 c2>>) /\
-      (<<EVENT: pf_event e>>)
-  .
-  Proof.
-    inv STEP. splits; auto. econs; eauto.
-    i. eapply pf_consistent_consistent; eauto.
-  Qed.
-
-  Lemma pf_step_future
-        e tid c1 c2
-        (STEP: pf_step e tid c1 c2)
-        (WF1: Configuration.wf c1)
-        (PF: pf_configuration c1):
-    (<<WF2: Configuration.wf c2>>) /\
-    (<<SC_FUTURE: TimeMap.le c1.(Configuration.sc) c2.(Configuration.sc)>>) /\
-    (<<MEM_FUTURE: Memory.future c1.(Configuration.memory) c2.(Configuration.memory)>>) /\
-    (<<PF: pf_configuration c2>>).
-  Proof.
-    exploit pf_step_pf_event_configuration_step; eauto. i. des.
-    exploit SConfiguration.step_future; eauto. i. des.
-    splits; auto. eapply pf_configuration_step; eauto.
-  Qed.
-
-  Lemma pf_machine_step_future
-        e tid c1 c2
-        (STEP: pf_machine_step e tid c1 c2)
-        (WF1: Configuration.wf c1)
-        (PF: pf_configuration c1):
-    (<<WF2: Configuration.wf c2>>) /\
-    (<<SC_FUTURE: TimeMap.le c1.(Configuration.sc) c2.(Configuration.sc)>>) /\
-    (<<MEM_FUTURE: Memory.future c1.(Configuration.memory) c2.(Configuration.memory)>>) /\
-    (<<PF: pf_configuration c2>>).
-  Proof.
-    inv STEP. eapply pf_step_future; eauto.
-  Qed.
-
-  Lemma opt_pf_machine_step_future
-        e tid c1 c2
-        (STEP: opt_pf_machine_step e tid c1 c2)
-        (WF1: Configuration.wf c1)
-        (PF: pf_configuration c1):
-    (<<WF2: Configuration.wf c2>>) /\
-    (<<SC_FUTURE: TimeMap.le c1.(Configuration.sc) c2.(Configuration.sc)>>) /\
-    (<<MEM_FUTURE: Memory.future c1.(Configuration.memory) c2.(Configuration.memory)>>) /\
-    (<<PF: pf_configuration c2>>).
-  Proof.
-    inv STEP; eauto.
-    - splits; eauto. refl.
-    - eapply pf_machine_step_future; eauto.
-  Qed.
-
-  Lemma pf_all_step_future
-        c1 c2
-        (STEP: pf_all_step c1 c2)
-        (WF1: Configuration.wf c1)
-        (PF: pf_configuration c1):
-    (<<WF2: Configuration.wf c2>>) /\
-    (<<SC_FUTURE: TimeMap.le c1.(Configuration.sc) c2.(Configuration.sc)>>) /\
-    (<<MEM_FUTURE: Memory.future c1.(Configuration.memory) c2.(Configuration.memory)>>) /\
-    (<<PF: pf_configuration c2>>).
-  Proof.
-    inv STEP. eapply pf_step_future; eauto.
-  Qed.
-
-  Lemma tau_pf_machine_step_future
-        c1 c2
-        (STEP: tau_pf_machine_step c1 c2)
-        (WF1: Configuration.wf c1)
-        (PF: pf_configuration c1):
-    (<<WF2: Configuration.wf c2>>) /\
-    (<<SC_FUTURE: TimeMap.le c1.(Configuration.sc) c2.(Configuration.sc)>>) /\
-    (<<MEM_FUTURE: Memory.future c1.(Configuration.memory) c2.(Configuration.memory)>>) /\
-    (<<PF: pf_configuration c2>>).
-  Proof.
-    inv STEP. eapply pf_machine_step_future; eauto.
-  Qed.
-
-  Lemma rtc_tau_pf_machine_step_future
-        c1 c2
-        (STEPS: rtc tau_pf_machine_step c1 c2)
-        (WF1: Configuration.wf c1)
-        (PF: pf_configuration c1):
-    (<<WF2: Configuration.wf c2>>) /\
-    (<<SC_FUTURE: TimeMap.le c1.(Configuration.sc) c2.(Configuration.sc)>>) /\
-    (<<MEM_FUTURE: Memory.future c1.(Configuration.memory) c2.(Configuration.memory)>>) /\
-    (<<PF: pf_configuration c2>>).
-  Proof.
-    ginduction STEPS; eauto.
-    - i. splits; eauto. refl.
-    - i. exploit tau_pf_machine_step_future; eauto. i. des.
-      exploit IHSTEPS; eauto. i. des. esplits; eauto. etrans; eauto.
-  Qed.
-
-  Lemma rtc_pf_all_step_future
-        c1 c2
-        (STEPS: rtc pf_all_step c1 c2)
-        (WF1: Configuration.wf c1)
-        (PF: pf_configuration c1):
-    (<<WF2: Configuration.wf c2>>) /\
-    (<<SC_FUTURE: TimeMap.le c1.(Configuration.sc) c2.(Configuration.sc)>>) /\
-    (<<MEM_FUTURE: Memory.future c1.(Configuration.memory) c2.(Configuration.memory)>>) /\
-    (<<PF: pf_configuration c2>>).
-Proof.
-    ginduction STEPS; eauto.
-    - i. splits; eauto. refl.
-    - i. exploit pf_all_step_future; eauto. i. des.
-      exploit IHSTEPS; eauto. i. des. esplits; eauto. etrans; eauto.
-  Qed.
-
-  Lemma pf_steps_future
-        es tid c1 c2
-        (STEPS: pf_steps es tid c1 c2)
-        (WF1: Configuration.wf c1)
-        (PF: pf_configuration c1):
-    (<<WF2: Configuration.wf c2>>) /\
-    (<<SC_FUTURE: TimeMap.le c1.(Configuration.sc) c2.(Configuration.sc)>>) /\
-    (<<MEM_FUTURE: Memory.future c1.(Configuration.memory) c2.(Configuration.memory)>>) /\
-    (<<PF: pf_configuration c2>>).
-  Proof.
-    ginduction STEPS; eauto.
-    - i. splits; eauto. refl.
-    - i. exploit pf_step_future; eauto. i. des.
-      exploit IHSTEPS; eauto. i. des. esplits; eauto. etrans; eauto.
-  Qed.
-
-  Inductive pf_step_trace: forall (tr: Trace.t) (e:MachineEvent.t) (tid:Ident.t) (c1 c2:Configuration.t), Prop :=
-  | pf_step_trace_intro
-      lang tr e tr' pf tid c1 st1 lc1 e2 st3 lc3 sc3 memory3
-      (TID: IdentMap.find tid c1.(Configuration.threads) = Some (existT _ lang st1, lc1))
-      (STEPS: Trace.steps tr' (Thread.mk _ st1 lc1 c1.(Configuration.sc) c1.(Configuration.memory)) e2)
-      (SILENT: List.Forall (fun the => ThreadEvent.get_machine_event (snd the) = MachineEvent.silent) tr')
-      (STEP: Thread.step pf e e2 (Thread.mk _ st3 lc3 sc3 memory3))
-      (TR: tr = tr'++[(e2.(Thread.local), e)])
-      (CONSISTENT: forall (EVENT: e <> ThreadEvent.failure),
-          pf_consistent (Thread.mk _ st3 lc3 sc3 memory3))
-      (PF: List.Forall (compose pf_event snd) tr)
-    :
-      pf_step_trace tr (ThreadEvent.get_machine_event e) tid c1 (Configuration.mk (IdentMap.add tid (existT _ _ st3, lc3) c1.(Configuration.threads)) sc3 memory3)
-  .
 
   Lemma pf_promises_trace_steps lang (th0 th1: Thread.t lang) tr
         (STEPS: Trace.steps tr th0 th1)
@@ -619,48 +216,362 @@ Proof.
     eapply pf_promises_step; eauto.
   Qed.
 
-  Lemma pf_trace_step_pf_step_trace c1 c2 tr e tid
+  Lemma pf_promises_consistent_consistent lang (th: Thread.t lang)
+        (CONSISTENT: Thread.consistent th)
+        (WF: Local.wf th.(Thread.local) th.(Thread.memory))
+        (MEM: Memory.closed th.(Thread.memory))
+        (PROMISES: pf_promises th.(Thread.local).(Local.promises))
+    :
+      pf_consistent th.
+  Proof.
+    eapply consistent_pf_consistent in CONSISTENT; eauto.
+    exploit Memory.cap_exists; eauto. i. des.
+    exploit Memory.max_concrete_timemap_exists.
+    { eapply Memory.cap_closed; eauto. } i. des.
+    exploit CONSISTENT; eauto. i. des.
+    { eapply pf_promises_steps_trace in STEPS; eauto. des.
+      exists tr. splits; auto. ii.
+      exploit (@Memory.cap_inj th.(Thread.memory) mem2 mem1); eauto. i. subst.
+      exploit (@Memory.max_concrete_timemap_inj mem1 tm sc1); eauto. i. subst.
+      esplits; eauto.
+    }
+    { eapply pf_promises_steps_trace in STEPS; eauto. des.
+      exists tr. splits; auto. ii.
+      exploit (@Memory.cap_inj th.(Thread.memory) mem2 mem1); eauto. i. subst.
+      exploit (@Memory.max_concrete_timemap_inj mem1 tm sc1); eauto. i. subst.
+      esplits; eauto.
+    }
+  Qed.
+End LOCALPF.
+End PF.
+
+(** L-PF machine **)
+Module PFConfiguration.
+Section LOCALPF.
+  Variable L: Loc.t -> bool.
+
+  Inductive step:
+    forall (e:ThreadEvent.t) (tid:Ident.t) (c1 c2:Configuration.t), Prop :=
+  | step_intro
+      e tid c1 lang st1 lc1 e2 e3 st4 lc4 sc4 memory4
+      (TID: IdentMap.find tid c1.(Configuration.threads) = Some (existT _ lang st1, lc1))
+      (CANCELS: rtc (@Thread.cancel_step _) (Thread.mk _ st1 lc1 c1.(Configuration.sc) c1.(Configuration.memory)) e2)
+      (STEP: Thread.opt_step e e2 e3)
+      (RESERVES: rtc (@Thread.reserve_step _) e3 (Thread.mk _ st4 lc4 sc4 memory4))
+      (CONSISTENT: e <> ThreadEvent.failure -> PF.pf_consistent L (Thread.mk _ st4 lc4 sc4 memory4))
+      (PF: PF.pf_event L e)
+    :
+      step e tid c1 (Configuration.mk (IdentMap.add tid (existT _ _ st4, lc4) c1.(Configuration.threads)) sc4 memory4)
+  .
+  Hint Constructors step.
+
+  Inductive machine_step: forall (e:MachineEvent.t) (tid:Ident.t) (c1 c2:Configuration.t), Prop :=
+  | machine_step_intro
+      e tid c1 c2
+      (STEP: step e tid c1 c2)
+    :
+      machine_step (ThreadEvent.get_machine_event e) tid c1 c2
+  .
+  Hint Constructors machine_step.
+
+  Inductive all_step (c1 c2: Configuration.t): Prop :=
+  | all_step_intro
+      e tid
+      (STEP: step e tid c1 c2)
+  .
+  Hint Constructors all_step.
+
+  (** Properties of the L-PF machine **)
+  Inductive opt_machine_step:
+    forall (e: MachineEvent.t) (tid: Ident.t) (c1 c2: Configuration.t), Prop :=
+  | opt_machine_step_none
+      tid c:
+      opt_machine_step MachineEvent.silent tid c c
+  | opt_machine_step_some
+      e tid c1 c2
+      (STEP: machine_step e tid c1 c2):
+      opt_machine_step e tid c1 c2
+  .
+  Hint Constructors opt_machine_step.
+
+  Definition tau_machine_step := union (machine_step MachineEvent.silent).
+
+  Inductive steps:
+    forall (es: list ThreadEvent.t) (tid: Ident.t) (c1 c2:Configuration.t), Prop :=
+  | steps_nil
+      tid c1
+    :
+      steps [] tid c1 c1
+  | steps_cons
+      ehd etl tid c1 c2 c3
+      (STEP: step ehd tid c1 c2)
+      (STEPS: steps etl tid c2 c3)
+    :
+      steps (ehd :: etl) tid c1 c3
+  .
+  Hint Constructors steps.
+
+  Lemma steps_rtc_all_step es tid c1 c2
+        (STEPS: steps es tid c1 c2)
+    :
+      rtc all_step c1 c2.
+  Proof.
+    induction STEPS; eauto.
+  Qed.
+
+  Lemma steps_split es0 es1 tid c0 c2
+        (STEPS: steps (es0 ++ es1) tid c0 c2)
+    :
+      exists c1,
+        (<<STEPS0: steps es0 tid c0 c1>>) /\
+        (<<STEPS1: steps es1 tid c1 c2>>).
+  Proof.
+    ginduction es0; eauto. i. ss. inv STEPS.
+    exploit IHes0; eauto. i. des.
+    esplits; eauto.
+  Qed.
+
+  Lemma silent_steps_tau_machine_steps es tid c1 c2
+        (STEPS: steps es tid c1 c2)
+        (SILENT: List.Forall (fun e => ThreadEvent.get_machine_event e = MachineEvent.silent) es)
+    :
+      rtc (machine_step MachineEvent.silent tid) c1 c2.
+  Proof.
+    ginduction es; i.
+    { inv STEPS. eauto. }
+    { inv STEPS. inv SILENT. exploit IHes; eauto.
+      i. econs 2; eauto. rewrite <- H1. econs; eauto. }
+  Qed.
+
+  Lemma pf_configuration_step tid c1 c2 e
+        (STEP: step e tid c1 c2)
+        (PF: PF.pf_configuration L c1)
+    :
+      PF.pf_configuration L c2.
+  Proof.
+    inv STEP. unfold PF.pf_configuration in *. i. ss.
+    erewrite IdentMap.gsspec in TID0. des_ifs; eauto.
+    dep_clarify. eapply PF in TID.
+    eapply PF.pf_promises_cancel_steps in CANCELS; eauto.
+    eapply PF.pf_promises_opt_step in STEP0; eauto.
+    eapply PF.pf_promises_reserve_steps in RESERVES; eauto.
+  Qed.
+
+  Lemma event_configuration_step_step c1 c2 e tid
+        (STEP: SConfiguration.step e tid c1 c2)
+        (WF: Configuration.wf c1)
+        (PF: PF.pf_configuration L c1)
+        (EVENT: PF.pf_event L e)
+    :
+      step e tid c1 c2.
+  Proof.
+    inv STEP. econs; eauto. i.
+    exploit Thread.rtc_cancel_step_future; eauto; try eapply WF; eauto. ss. i. des.
+    exploit Thread.opt_step_future; eauto. ss. i. des.
+    exploit Thread.rtc_reserve_step_future; eauto; try eapply WF; eauto. ss. i. des.
+    hexploit PF.pf_promises_cancel_steps; eauto. i. ss.
+    hexploit PF.pf_promises_opt_step; eauto. i. ss.
+    hexploit PF.pf_promises_reserve_steps; eauto. i. ss.
+    eapply PF.pf_promises_consistent_consistent; eauto.
+  Qed.
+
+  Lemma reservation_only_step_step tid c1 c2
+        (STEP: SConfiguration.reservation_only_step tid c1 c2)
+        (WF: Configuration.wf c1)
+        (PF: PF.pf_configuration L c1)
+    :
+      step ThreadEvent.silent tid c1 c2.
+  Proof.
+    eapply SConfiguration.reservation_only_step_step in STEP.
+    eapply event_configuration_step_step; eauto. ss.
+  Qed.
+
+  Lemma step_event_configuration_step c1 c2 e tid
+        (STEP: step e tid c1 c2)
+        (WF: Configuration.wf c1)
+    :
+      (<<STEP: SConfiguration.step e tid c1 c2>>) /\
+      (<<EVENT: PF.pf_event L e>>)
+  .
+  Proof.
+    inv STEP. splits; auto. econs; eauto.
+    i. eapply PF.pf_consistent_consistent; eauto.
+  Qed.
+
+  Lemma step_future
+        e tid c1 c2
+        (STEP: step e tid c1 c2)
+        (WF1: Configuration.wf c1)
+        (PF: PF.pf_configuration L c1):
+    (<<WF2: Configuration.wf c2>>) /\
+    (<<SC_FUTURE: TimeMap.le c1.(Configuration.sc) c2.(Configuration.sc)>>) /\
+    (<<MEM_FUTURE: Memory.future c1.(Configuration.memory) c2.(Configuration.memory)>>) /\
+    (<<PF: PF.pf_configuration L c2>>).
+  Proof.
+    exploit step_event_configuration_step; eauto. i. des.
+    exploit SConfiguration.step_future; eauto. i. des.
+    splits; auto. eapply pf_configuration_step; eauto.
+  Qed.
+
+  Lemma machine_step_future
+        e tid c1 c2
+        (STEP: machine_step e tid c1 c2)
+        (WF1: Configuration.wf c1)
+        (PF: PF.pf_configuration L c1):
+    (<<WF2: Configuration.wf c2>>) /\
+    (<<SC_FUTURE: TimeMap.le c1.(Configuration.sc) c2.(Configuration.sc)>>) /\
+    (<<MEM_FUTURE: Memory.future c1.(Configuration.memory) c2.(Configuration.memory)>>) /\
+    (<<PF: PF.pf_configuration L c2>>).
+  Proof.
+    inv STEP. eapply step_future; eauto.
+  Qed.
+
+  Lemma opt_machine_step_future
+        e tid c1 c2
+        (STEP: opt_machine_step e tid c1 c2)
+        (WF1: Configuration.wf c1)
+        (PF: PF.pf_configuration L c1):
+    (<<WF2: Configuration.wf c2>>) /\
+    (<<SC_FUTURE: TimeMap.le c1.(Configuration.sc) c2.(Configuration.sc)>>) /\
+    (<<MEM_FUTURE: Memory.future c1.(Configuration.memory) c2.(Configuration.memory)>>) /\
+    (<<PF: PF.pf_configuration L c2>>).
+  Proof.
+    inv STEP; eauto.
+    - splits; eauto. refl.
+    - eapply machine_step_future; eauto.
+  Qed.
+
+  Lemma all_step_future
+        c1 c2
+        (STEP: all_step c1 c2)
+        (WF1: Configuration.wf c1)
+        (PF: PF.pf_configuration L c1):
+    (<<WF2: Configuration.wf c2>>) /\
+    (<<SC_FUTURE: TimeMap.le c1.(Configuration.sc) c2.(Configuration.sc)>>) /\
+    (<<MEM_FUTURE: Memory.future c1.(Configuration.memory) c2.(Configuration.memory)>>) /\
+    (<<PF: PF.pf_configuration L c2>>).
+  Proof.
+    inv STEP. eapply step_future; eauto.
+  Qed.
+
+  Lemma tau_machine_step_future
+        c1 c2
+        (STEP: tau_machine_step c1 c2)
+        (WF1: Configuration.wf c1)
+        (PF: PF.pf_configuration L c1):
+    (<<WF2: Configuration.wf c2>>) /\
+    (<<SC_FUTURE: TimeMap.le c1.(Configuration.sc) c2.(Configuration.sc)>>) /\
+    (<<MEM_FUTURE: Memory.future c1.(Configuration.memory) c2.(Configuration.memory)>>) /\
+    (<<PF: PF.pf_configuration L c2>>).
+  Proof.
+    inv STEP. eapply machine_step_future; eauto.
+  Qed.
+
+  Lemma rtc_tau_machine_step_future
+        c1 c2
+        (STEPS: rtc tau_machine_step c1 c2)
+        (WF1: Configuration.wf c1)
+        (PF: PF.pf_configuration L c1):
+    (<<WF2: Configuration.wf c2>>) /\
+    (<<SC_FUTURE: TimeMap.le c1.(Configuration.sc) c2.(Configuration.sc)>>) /\
+    (<<MEM_FUTURE: Memory.future c1.(Configuration.memory) c2.(Configuration.memory)>>) /\
+    (<<PF: PF.pf_configuration L c2>>).
+  Proof.
+    ginduction STEPS; eauto.
+    - i. splits; eauto. refl.
+    - i. exploit tau_machine_step_future; eauto. i. des.
+      exploit IHSTEPS; eauto. i. des. esplits; eauto. etrans; eauto.
+  Qed.
+
+  Lemma rtc_all_step_future
+        c1 c2
+        (STEPS: rtc all_step c1 c2)
+        (WF1: Configuration.wf c1)
+        (PF: PF.pf_configuration L c1):
+    (<<WF2: Configuration.wf c2>>) /\
+    (<<SC_FUTURE: TimeMap.le c1.(Configuration.sc) c2.(Configuration.sc)>>) /\
+    (<<MEM_FUTURE: Memory.future c1.(Configuration.memory) c2.(Configuration.memory)>>) /\
+    (<<PF: PF.pf_configuration L c2>>).
+Proof.
+    ginduction STEPS; eauto.
+    - i. splits; eauto. refl.
+    - i. exploit all_step_future; eauto. i. des.
+      exploit IHSTEPS; eauto. i. des. esplits; eauto. etrans; eauto.
+  Qed.
+
+  Lemma steps_future
+        es tid c1 c2
+        (STEPS: steps es tid c1 c2)
+        (WF1: Configuration.wf c1)
+        (PF: PF.pf_configuration L c1):
+    (<<WF2: Configuration.wf c2>>) /\
+    (<<SC_FUTURE: TimeMap.le c1.(Configuration.sc) c2.(Configuration.sc)>>) /\
+    (<<MEM_FUTURE: Memory.future c1.(Configuration.memory) c2.(Configuration.memory)>>) /\
+    (<<PF: PF.pf_configuration L c2>>).
+  Proof.
+    ginduction STEPS; eauto.
+    - i. splits; eauto. refl.
+    - i. exploit step_future; eauto. i. des.
+      exploit IHSTEPS; eauto. i. des. esplits; eauto. etrans; eauto.
+  Qed.
+
+  Inductive step_trace: forall (tr: Trace.t) (e:MachineEvent.t) (tid:Ident.t) (c1 c2:Configuration.t), Prop :=
+  | step_trace_intro
+      lang tr e tr' pf tid c1 st1 lc1 e2 st3 lc3 sc3 memory3
+      (TID: IdentMap.find tid c1.(Configuration.threads) = Some (existT _ lang st1, lc1))
+      (STEPS: Trace.steps tr' (Thread.mk _ st1 lc1 c1.(Configuration.sc) c1.(Configuration.memory)) e2)
+      (SILENT: List.Forall (fun the => ThreadEvent.get_machine_event (snd the) = MachineEvent.silent) tr')
+      (STEP: Thread.step pf e e2 (Thread.mk _ st3 lc3 sc3 memory3))
+      (TR: tr = tr'++[(e2.(Thread.local), e)])
+      (CONSISTENT: forall (EVENT: e <> ThreadEvent.failure),
+          PF.pf_consistent L (Thread.mk _ st3 lc3 sc3 memory3))
+      (PF: List.Forall (compose (PF.pf_event L) snd) tr)
+    :
+      step_trace tr (ThreadEvent.get_machine_event e) tid c1 (Configuration.mk (IdentMap.add tid (existT _ _ st3, lc3) c1.(Configuration.threads)) sc3 memory3)
+  .
+
+  Lemma trace_step_step_trace c1 c2 tr e tid
         (STEP: Trace.configuration_step tr e tid c1 c2)
         (WF: Configuration.wf c1)
-        (PF: pf_configuration c1)
-        (TRACE: List.Forall (compose pf_event snd) tr)
+        (PF: PF.pf_configuration L c1)
+        (TRACE: List.Forall (compose (PF.pf_event L) snd) tr)
     :
-      pf_step_trace tr e tid c1 c2.
+      step_trace tr e tid c1 c2.
   Proof.
     inv STEP. econs; eauto. i.
     eapply Forall_app_inv in TRACE. des. inv FORALL2.
     exploit Trace.steps_future; eauto; try eapply WF; eauto. ss. i. des.
     exploit Thread.step_future; eauto. ss. i. des.
-    hexploit pf_promises_trace_steps; eauto. i. ss.
-    hexploit pf_promises_step; eauto. i. ss.
-    eapply pf_promises_consistent_pf_consistent; eauto.
+    hexploit PF.pf_promises_trace_steps; eauto. i. ss.
+    hexploit PF.pf_promises_step; eauto. i. ss.
+    eapply PF.pf_promises_consistent_consistent; eauto.
   Qed.
 
-  Lemma pf_step_trace_pf_trace_step c1 c2 tr e tid
-        (STEP: pf_step_trace tr e tid c1 c2)
+  Lemma step_trace_trace_step c1 c2 tr e tid
+        (STEP: step_trace tr e tid c1 c2)
         (WF: Configuration.wf c1)
     :
       (<<STEP: Trace.configuration_step tr e tid c1 c2>>) /\
-      (<<TRACE: List.Forall (compose pf_event snd) tr>>).
+      (<<TRACE: List.Forall (compose (PF.pf_event L) snd) tr>>).
   Proof.
     inv STEP. splits; auto. econs; eauto. i.
-    eapply pf_consistent_consistent; eauto.
+    eapply PF.pf_consistent_consistent; eauto.
   Qed.
 
-  Inductive pf_opt_step_trace: forall (tr: Trace.t) (e:MachineEvent.t) (tid:Ident.t) (c1 c2:Configuration.t), Prop :=
-  | pf_opt_step_trace_some
+  Inductive opt_step_trace: forall (tr: Trace.t) (e:MachineEvent.t) (tid:Ident.t) (c1 c2:Configuration.t), Prop :=
+  | opt_step_trace_some
       tr e tid c1 c2
-      (STEP: pf_step_trace tr e tid c1 c2)
+      (STEP: step_trace tr e tid c1 c2)
     :
-      pf_opt_step_trace tr e tid c1 c2
-  | pf_opt_step_trace_none
+      opt_step_trace tr e tid c1 c2
+  | opt_step_trace_none
       tid c1
     :
-      pf_opt_step_trace [] MachineEvent.silent tid c1 c1
+      opt_step_trace [] MachineEvent.silent tid c1 c1
   .
 
-  Lemma pf_step_trace_step tr e tid c1 c2
-        (STEP: pf_step_trace tr e tid c1 c2)
+  Lemma step_trace_step tr e tid c1 c2
+        (STEP: step_trace tr e tid c1 c2)
     :
       Configuration.step e tid c1 c2.
   Proof.
@@ -669,104 +580,104 @@ Proof.
       eapply Trace.silent_steps_tau_steps; eauto. }
     { econs 2; try apply STEP0; eauto.
       { eapply Trace.silent_steps_tau_steps; eauto. }
-      { exploit CONSISTENT; eauto. i. unfold pf_consistent in *. des.
+      { exploit CONSISTENT; eauto. i. unfold PF.pf_consistent in *. des.
         eapply Trace.consistent_thread_consistent; eauto. }
     }
   Qed.
 
-  Inductive pf_steps_trace:
+  Inductive steps_trace:
     forall (c0 c1: Configuration.t) (tr: Trace.t), Prop :=
-  | pf_steps_trace_nil
+  | steps_trace_nil
       c0
     :
-      pf_steps_trace c0 c0 []
-  | pf_steps_trace_cons
+      steps_trace c0 c0 []
+  | steps_trace_cons
       c0 c1 c2 trs tr e tid
-      (STEPS: pf_steps_trace c1 c2 trs)
-      (STEP: pf_step_trace tr e tid c0 c1)
+      (STEPS: steps_trace c1 c2 trs)
+      (STEP: step_trace tr e tid c0 c1)
     :
-      pf_steps_trace c0 c2 (tr ++ trs)
+      steps_trace c0 c2 (tr ++ trs)
   .
 
-  Lemma pf_step_trace_pf_steps tr e tid c1 c3
-        (STEP: pf_step_trace tr e tid c1 c3)
+  Lemma step_trace_steps tr e tid c1 c3
+        (STEP: step_trace tr e tid c1 c3)
         (WF: Configuration.wf c1)
-        (PF: pf_configuration c1)
+        (PF: PF.pf_configuration L c1)
     :
-      ((<<STEPS: pf_steps (List.filter ThreadEvent.is_normal_dec (List.map snd tr)) tid c1 c3>>) /\
+      ((<<STEPS: steps (List.filter ThreadEvent.is_normal_dec (List.map snd tr)) tid c1 c3>>) /\
        (<<NIL: List.filter ThreadEvent.is_normal_dec (List.map snd tr) <> []>>)) \/
       ((<<STEP: SConfiguration.reservation_only_step tid c1 c3>>) /\
        (<<NIL: List.filter ThreadEvent.is_normal_dec (List.map snd tr) = []>>)).
   Proof.
-    eapply pf_step_trace_pf_trace_step in STEP; eauto. des.
+    eapply step_trace_trace_step in STEP; eauto. des.
     eapply SConfiguration.trace_step_machine_step in STEP0; eauto. des; eauto.
     left. splits; auto. clear e.
     remember (List.filter (fun e => ThreadEvent.is_normal_dec e) (List.map snd tr)).
-    assert (EVENTS: List.Forall pf_event l).
+    assert (EVENTS: List.Forall (PF.pf_event L) l).
     { subst. clear - TRACE. induction tr; ss. inv TRACE. des_ifs; eauto. }
     clear tr Heql NIL TRACE. ginduction STEPS; eauto.
     i. inv EVENTS.
-    eapply pf_event_configuration_step_pf_step in STEP; eauto.
-    exploit pf_step_future; eauto. i. des.
+    eapply event_configuration_step_step in STEP; eauto.
+    exploit step_future; eauto. i. des.
     hexploit pf_configuration_step; eauto.
   Qed.
 
-  Lemma pf_step_trace_future
+  Lemma step_trace_future
         (tr: Trace.t) e tid c1 c2
-        (STEP: pf_step_trace tr e tid c1 c2)
+        (STEP: step_trace tr e tid c1 c2)
         (WF1: Configuration.wf c1)
-        (PF: pf_configuration c1):
+        (PF: PF.pf_configuration L c1):
     (<<WF2: Configuration.wf c2>>) /\
     (<<SC_FUTURE: TimeMap.le c1.(Configuration.sc) c2.(Configuration.sc)>>) /\
     (<<MEM_FUTURE: Memory.future c1.(Configuration.memory) c2.(Configuration.memory)>>) /\
-    (<<PF: pf_configuration c2>>).
+    (<<PF: PF.pf_configuration L c2>>).
   Proof.
-    eapply pf_step_trace_pf_steps in STEP; eauto. des.
-    { eapply pf_steps_future; eauto. }
-    { eapply reservation_only_step_pf_step in STEP0; eauto.
-      eapply pf_step_future; eauto. }
+    eapply step_trace_steps in STEP; eauto. des.
+    { eapply steps_future; eauto. }
+    { eapply reservation_only_step_step in STEP0; eauto.
+      eapply step_future; eauto. }
   Qed.
 
-  Lemma pf_opt_step_trace_future
+  Lemma opt_step_trace_future
         (tr: Trace.t) e tid c1 c2
-        (STEP: pf_opt_step_trace tr e tid c1 c2)
+        (STEP: opt_step_trace tr e tid c1 c2)
         (WF1: Configuration.wf c1)
-        (PF: pf_configuration c1):
+        (PF: PF.pf_configuration L c1):
     (<<WF2: Configuration.wf c2>>) /\
     (<<SC_FUTURE: TimeMap.le c1.(Configuration.sc) c2.(Configuration.sc)>>) /\
     (<<MEM_FUTURE: Memory.future c1.(Configuration.memory) c2.(Configuration.memory)>>) /\
-    (<<PF: pf_configuration c2>>).
+    (<<PF: PF.pf_configuration L c2>>).
   Proof.
     inv STEP.
-    { eapply pf_step_trace_future; eauto. }
+    { eapply step_trace_future; eauto. }
     { splits; auto. refl. }
   Qed.
 
-  Lemma pf_steps_trace_future
+  Lemma steps_trace_future
         c1 c2 tr
-        (STEPS: pf_steps_trace c1 c2 tr)
+        (STEPS: steps_trace c1 c2 tr)
         (WF1: Configuration.wf c1)
-        (PF: pf_configuration c1):
+        (PF: PF.pf_configuration L c1):
     (<<WF2: Configuration.wf c2>>) /\
     (<<SC_FUTURE: TimeMap.le c1.(Configuration.sc) c2.(Configuration.sc)>>) /\
     (<<MEM_FUTURE: Memory.future c1.(Configuration.memory) c2.(Configuration.memory)>>) /\
-    (<<PF: pf_configuration c2>>).
+    (<<PF: PF.pf_configuration L c2>>).
   Proof.
     revert WF1. induction STEPS; i.
     - splits; ss; refl.
-    - exploit pf_step_trace_future; eauto. i. des.
+    - exploit step_trace_future; eauto. i. des.
       exploit IHSTEPS; eauto. i. des.
       splits; ss; etrans; eauto.
   Qed.
 
-  Lemma pf_steps_trace_n1 c0 c1 c2 tr trs e tid
-        (STEPS: pf_steps_trace c0 c1 trs)
-        (STEP: pf_step_trace tr e tid c1 c2)
+  Lemma steps_trace_n1 c0 c1 c2 tr trs e tid
+        (STEPS: steps_trace c0 c1 trs)
+        (STEP: step_trace tr e tid c1 c2)
     :
-      pf_steps_trace c0 c2 (trs ++ tr).
+      steps_trace c0 c2 (trs ++ tr).
   Proof.
     ginduction STEPS.
-    { i. exploit pf_steps_trace_cons.
+    { i. exploit steps_trace_cons.
       { econs 1. }
       { eapply STEP. }
       { i. ss. erewrite List.app_nil_r in *. auto. }
@@ -774,78 +685,78 @@ Proof.
     { i. exploit IHSTEPS; eauto. i. erewrite <- List.app_assoc. econs; eauto. }
   Qed.
 
-  Lemma pf_steps_trace_trans c0 c1 c2 trs0 trs1
-        (STEPS0: pf_steps_trace c0 c1 trs0)
-        (STEPS1: pf_steps_trace c1 c2 trs1)
+  Lemma steps_trace_trans c0 c1 c2 trs0 trs1
+        (STEPS0: steps_trace c0 c1 trs0)
+        (STEPS1: steps_trace c1 c2 trs1)
     :
-      pf_steps_trace c0 c2 (trs0 ++ trs1).
+      steps_trace c0 c2 (trs0 ++ trs1).
   Proof.
     ginduction STEPS0.
     { i. erewrite List.app_nil_l. eauto. }
     { i. exploit IHSTEPS0; eauto. i. erewrite <- List.app_assoc. econs; eauto. }
   Qed.
 
-  Lemma pf_step_trace_pf_steps_trace tr e tid c1 c2
-        (STEP: pf_step_trace tr e tid c1 c2)
+  Lemma step_trace_steps_trace tr e tid c1 c2
+        (STEP: step_trace tr e tid c1 c2)
     :
-      pf_steps_trace c1 c2 tr.
+      steps_trace c1 c2 tr.
   Proof.
-    exploit pf_steps_trace_cons.
+    exploit steps_trace_cons.
     { econs 1. }
     { eauto. }
     i. rewrite List.app_nil_r in x0. auto.
   Qed.
 
-  Lemma pf_opt_step_trace_pf_steps_trace tr e tid c1 c2
-        (STEP: pf_opt_step_trace tr e tid c1 c2)
+  Lemma opt_step_trace_steps_trace tr e tid c1 c2
+        (STEP: opt_step_trace tr e tid c1 c2)
     :
-      pf_steps_trace c1 c2 tr.
+      steps_trace c1 c2 tr.
   Proof.
     inv STEP.
-    { eapply pf_step_trace_pf_steps_trace; eauto. }
+    { eapply step_trace_steps_trace; eauto. }
     { econs 1. }
   Qed.
 
-  Inductive silent_pf_steps_trace:
+  Inductive silent_steps_trace:
     forall (c0 c1: Configuration.t) (tr: Trace.t), Prop :=
-  | silent_pf_steps_trace_nil
+  | silent_steps_trace_nil
       c0
     :
-      silent_pf_steps_trace c0 c0 []
-  | silent_pf_steps_trace_cons
+      silent_steps_trace c0 c0 []
+  | silent_steps_trace_cons
       c0 c1 c2 trs tr tid
-      (STEPS: silent_pf_steps_trace c1 c2 trs)
-      (STEP: pf_step_trace tr MachineEvent.silent tid c0 c1)
+      (STEPS: silent_steps_trace c1 c2 trs)
+      (STEP: step_trace tr MachineEvent.silent tid c0 c1)
     :
-      silent_pf_steps_trace c0 c2 (tr ++ trs)
+      silent_steps_trace c0 c2 (tr ++ trs)
   .
 
-  Lemma silent_pf_steps_trace_pf_steps_trace
+  Lemma silent_steps_trace_steps_trace
     :
-      silent_pf_steps_trace <3= pf_steps_trace.
+      silent_steps_trace <3= steps_trace.
   Proof.
     intros. induction PR.
     { econs. }
     { econs; eauto. }
   Qed.
 
-  Inductive pf_steps_trace_rev: forall (c1 c2: Configuration.t) (tr: Trace.t), Prop :=
-  | pf_steps_trace_rev_nil
+  Inductive steps_trace_rev: forall (c1 c2: Configuration.t) (tr: Trace.t), Prop :=
+  | steps_trace_rev_nil
       c:
-      pf_steps_trace_rev c c []
-  | pf_steps_trace_rev_cons
+      steps_trace_rev c c []
+  | steps_trace_rev_cons
       c1 c2 c3 tr1 tr2 e tid
-      (STEPS: pf_steps_trace_rev c1 c2 tr1)
-      (STEP: pf_step_trace tr2 e tid c2 c3):
-      pf_steps_trace_rev c1 c3 (tr1 ++ tr2)
+      (STEPS: steps_trace_rev c1 c2 tr1)
+      (STEP: step_trace tr2 e tid c2 c3):
+      steps_trace_rev c1 c3 (tr1 ++ tr2)
   .
-  Hint Constructors pf_steps_trace_rev.
+  Hint Constructors steps_trace_rev.
 
-  Lemma pf_steps_trace_rev_1n
+  Lemma steps_trace_rev_1n
         c1 c2 c3 tr1 tr2 e tid
-        (STEP: pf_step_trace tr1 e tid c1 c2)
-        (STEPS: pf_steps_trace_rev c2 c3 tr2):
-    pf_steps_trace_rev c1 c3 (tr1 ++ tr2).
+        (STEP: step_trace tr1 e tid c1 c2)
+        (STEPS: steps_trace_rev c2 c3 tr2):
+    steps_trace_rev c1 c3 (tr1 ++ tr2).
   Proof.
     revert tr1 e tid c1 STEP. induction STEPS; i.
     - replace (tr1 ++ []) with ([] ++ tr1) by (rewrite List.app_nil_r; ss).
@@ -855,39 +766,39 @@ Proof.
       econs 2; eauto.
   Qed.
 
-  Lemma pf_steps_trace_equiv c1 c2 tr:
-    pf_steps_trace c1 c2 tr <-> pf_steps_trace_rev c1 c2 tr.
+  Lemma steps_trace_equiv c1 c2 tr:
+    steps_trace c1 c2 tr <-> steps_trace_rev c1 c2 tr.
   Proof.
     split; i.
     - induction H; eauto.
-      eapply pf_steps_trace_rev_1n; eauto.
+      eapply steps_trace_rev_1n; eauto.
     - induction H; [econs 1|].
-      eapply pf_steps_trace_n1; eauto.
+      eapply steps_trace_n1; eauto.
   Qed.
 
-  Lemma pf_steps_trace_inv
+  Lemma steps_trace_inv
         c1 c2 tr lc e
-        (STEPS: pf_steps_trace c1 c2 tr)
+        (STEPS: steps_trace c1 c2 tr)
         (WF: Configuration.wf c1)
-        (PF: pf_configuration c1)
+        (PF: PF.pf_configuration L c1)
         (TRACE: List.In (lc, e) tr):
     exists c tr1 tid lang st1 lc1,
-      (<<STEPS: pf_steps_trace c1 c tr1>>) /\
+      (<<STEPS: steps_trace c1 c tr1>>) /\
       (<<FIND: IdentMap.find tid c.(Configuration.threads) = Some (existT _ lang st1, lc1)>>) /\
       exists tr2 pf e2 e3,
         (<<THREAD_STEPS: Trace.steps tr2 (Thread.mk _ st1 lc1 c.(Configuration.sc) c.(Configuration.memory)) e2>>) /\
         (<<SILENT: List.Forall (fun the => ThreadEvent.get_machine_event (snd the) = MachineEvent.silent) tr2>>) /\
-        (<<PF: List.Forall (compose pf_event snd) tr2>>) /\
+        (<<PF: List.Forall (compose (PF.pf_event L) snd) tr2>>) /\
         (<<LC: e2.(Thread.local) = lc>>) /\
         (<<THREAD_STEP: Thread.step pf e e2 e3>>) /\
         (<<CONS: Local.promise_consistent e3.(Thread.local)>>).
   Proof.
-    rewrite pf_steps_trace_equiv in STEPS.
+    rewrite steps_trace_equiv in STEPS.
     induction STEPS; ss.
     apply List.in_app_or in TRACE. des; eauto.
     clear IHSTEPS. inv STEP.
     exists c2, tr1, tid, lang, st1, lc1.
-    rewrite <- pf_steps_trace_equiv in STEPS.
+    rewrite <- steps_trace_equiv in STEPS.
     splits; ss.
     apply List.in_app_or in TRACE. des; cycle 1.
     { inv TRACE; ss. inv H. esplits; eauto.
@@ -895,14 +806,14 @@ Proof.
       - destruct (classic (e = ThreadEvent.failure)).
         + subst. inv STEP0; inv STEP. inv LOCAL. inv LOCAL0. ss.
         + exploit CONSISTENT; eauto. i. inv x. des.
-          exploit pf_steps_trace_future; eauto. i. des.
+          exploit steps_trace_future; eauto. i. des.
           inv WF2. inv WF0. exploit THREADS; eauto. i.
           exploit Trace.steps_future; try exact STEPS0; eauto. s. i. des.
           exploit Thread.step_future; try exact STEP0; eauto. s. i. des.
           hexploit consistent_promise_consistent;
             try eapply Trace.consistent_thread_consistent; try exact CONSISTENT0; eauto.
     }
-    exploit pf_steps_trace_future; eauto. i. des.
+    exploit steps_trace_future; eauto. i. des.
     inv WF2. inv WF0. exploit THREADS; eauto. i. clear DISJOINT THREADS.
     exploit Trace.steps_inv; try exact STEPS0; eauto.
     { destruct (classic (e1 = ThreadEvent.failure)).
@@ -920,29 +831,29 @@ Proof.
       apply Forall_app_inv in FORALL1. des. ss.
   Qed.
 
-  Inductive pf_multi_step (e:MachineEvent.t) (tid:Ident.t) (c1 c2:Configuration.t): Prop :=
-  | pf_multi_step_intro
+  Inductive multi_step (e:MachineEvent.t) (tid:Ident.t) (c1 c2:Configuration.t): Prop :=
+  | multi_step_intro
       tr
-      (STEP: pf_step_trace tr e tid c1 c2)
+      (STEP: step_trace tr e tid c1 c2)
   .
 
-  Lemma pf_multi_step_machine_step e tid c1 c3
-        (STEP: pf_multi_step e tid c1 c3)
+  Lemma multi_step_machine_step e tid c1 c3
+        (STEP: multi_step e tid c1 c3)
         (WF: Configuration.wf c1)
-        (PF: pf_configuration c1)
+        (PF: PF.pf_configuration L c1)
     :
       exists c2,
-        (<<STEPS: rtc tau_pf_machine_step c1 c2>>) /\
-        (<<STEP: opt_pf_machine_step e tid c2 c3>>).
+        (<<STEPS: rtc tau_machine_step c1 c2>>) /\
+        (<<STEP: opt_machine_step e tid c2 c3>>).
   Proof.
-    inv STEP. exploit pf_step_trace_pf_steps; eauto. i. des.
+    inv STEP. exploit step_trace_steps; eauto. i. des.
     { inv STEP0.
       rewrite List.map_app in *.
       rewrite list_filter_app in *. ss.
-      eapply pf_steps_split in STEPS. des. exists c0. splits.
-      { eapply rtc_implies with (R1:=(pf_machine_step MachineEvent.silent tid)).
+      eapply steps_split in STEPS. des. exists c0. splits.
+      { eapply rtc_implies with (R1:=(machine_step MachineEvent.silent tid)).
         { clear. i. econs; eauto. }
-        eapply silent_pf_steps_tau_pf_machine_steps; eauto.
+        eapply silent_steps_tau_machine_steps; eauto.
         eapply list_filter_forall with (Q:=fun e => ThreadEvent.get_machine_event e = MachineEvent.silent); eauto.
         eapply list_map_forall; eauto.
       }
@@ -957,7 +868,7 @@ Proof.
       }
     }
     { eapply SConfiguration.reservation_only_step_step in STEP.
-      eapply pf_event_configuration_step_pf_step in STEP; eauto; ss.
+      eapply event_configuration_step_step in STEP; eauto; ss.
       exists c1. esplits; eauto.
       replace e with (ThreadEvent.get_machine_event ThreadEvent.silent); eauto.
       ss. inv STEP0.
@@ -971,126 +882,226 @@ Proof.
     }
   Qed.
 
-  Lemma pf_multi_step_future
+  Lemma multi_step_future
         e tid c1 c2
-        (STEP: pf_multi_step e tid c1 c2)
+        (STEP: multi_step e tid c1 c2)
         (WF1: Configuration.wf c1)
-        (PF: pf_configuration c1):
+        (PF: PF.pf_configuration L c1):
     (<<WF2: Configuration.wf c2>>) /\
     (<<SC_FUTURE: TimeMap.le c1.(Configuration.sc) c2.(Configuration.sc)>>) /\
     (<<MEM_FUTURE: Memory.future c1.(Configuration.memory) c2.(Configuration.memory)>>) /\
-    (<<PF: pf_configuration c2>>).
+    (<<PF: PF.pf_configuration L c2>>).
   Proof.
-    inv STEP. eapply pf_step_trace_future; eauto.
+    inv STEP. eapply step_trace_future; eauto.
   Qed.
 
-  Lemma silent_pf_multi_steps_trace_behaviors c0 c1 tr
-        (STEP: silent_pf_steps_trace c0 c1 tr)
+  Lemma silent_multi_steps_trace_behaviors c0 c1 tr
+        (STEP: silent_steps_trace c0 c1 tr)
     :
-      behaviors pf_multi_step c1 <1= behaviors pf_multi_step c0.
+      behaviors multi_step c1 <1= behaviors multi_step c0.
   Proof.
     ginduction STEP; auto.
     i. eapply IHSTEP in PR. econs 4; eauto.
     econs. esplits; eauto.
   Qed.
 
-  Inductive pf_multi_race (c0: Configuration.t): Prop :=
-  | pf_multi_race_intro
-      c1
+  Lemma multi_step_behavior c
+        (WF: Configuration.wf c)
+        (PF: PF.pf_configuration L c)
+    :
+      behaviors multi_step c <1= behaviors machine_step c.
+  Proof.
+    i. induction PR.
+    - econs 1; eauto.
+    - exploit multi_step_future; eauto. i. des.
+      eapply multi_step_machine_step in STEP; eauto. des.
+      eapply rtc_tau_step_behavior; eauto.
+      inv STEP0; eauto. econs 2; eauto.
+    - exploit multi_step_future; eauto. i. des.
+      eapply multi_step_machine_step in STEP; eauto. des.
+      eapply rtc_tau_step_behavior; eauto.
+      inv STEP0; eauto. econs 3; eauto.
+    - exploit multi_step_future; eauto. i. des.
+      eapply multi_step_machine_step in STEP; eauto. des.
+      eapply rtc_tau_step_behavior; eauto.
+      inv STEP0; eauto. econs 4; eauto.
+  Qed.
+
+End LOCALPF.
+End PFConfiguration.
+
+
+Module PFRace.
+Section LOCALPFRACE.
+  Variable L: Loc.t -> bool.
+
+  (** The Definition of an L-PF race **)
+  Inductive reading_event (loc: Loc.t) (ts: Time.t):
+    forall (e: ThreadEvent.t), Prop :=
+  | reading_event_read
+      valr releasedr ordr
+    :
+      reading_event loc ts (ThreadEvent.read loc ts valr releasedr ordr)
+  | reading_event_update
+      to valr valw releasedr releasedw ordr ordw
+    :
+      reading_event loc ts (ThreadEvent.update loc ts to valr valw releasedr releasedw ordr ordw)
+  .
+
+  Inductive writing_event (loc: Loc.t) (ts: Time.t):
+    forall (e: ThreadEvent.t), Prop :=
+  | writing_event_write
+      from valw releasedw ordw
+      (ORD: Ordering.le ordw Ordering.relaxed)
+    :
+      writing_event loc ts (ThreadEvent.write loc from ts valw releasedw ordw)
+  | writing_event_update
+      from valr valw releasedr releasedw ordr ordw
+      (ORD: Ordering.le ordw Ordering.relaxed)
+    :
+      writing_event loc ts (ThreadEvent.update loc from ts valr valw releasedr releasedw ordr ordw)
+  .
+
+  Definition racy_execution (c0: Configuration.t): Prop :=
+    forall tid0 c1 tid1 c2 c3
+           loc ts e0 e1
+           (LOC: L loc)
+           (TID: tid0 <> tid1)
+           (CSTEP0: PFConfiguration.step L e0 tid0 c0 c1)
+           (WRITE: writing_event loc ts e0)
+           (STEPS: rtc (PFConfiguration.machine_step L MachineEvent.silent tid1) c1 c2)
+           (CSTEP1: PFConfiguration.step L e1 tid1 c2 c3)
+           (READ: reading_event loc ts e1),
+      False.
+
+  Definition racefree (c0: Configuration.t): Prop :=
+    forall c1
+           (CSTEPS: rtc (PFConfiguration.all_step L) c0 c1),
+      racy_execution c1.
+
+  Inductive racy_state (c0: Configuration.t): Prop :=
+  | race_intro
+      c1 c2
       tid0 tid1 e0 e1
       lang st0 lc0 th1 th2
-      e trs tr pf loc ts
-      (STEPS: pf_step_trace trs e tid0 c0 c1)
-      (TRACE: final_event_trace e0 trs)
+      tr pf loc ts
+      (STEPS: rtc (PFConfiguration.machine_step L MachineEvent.silent tid0) c0 c1)
+      (WRITE_STEP: PFConfiguration.step L e0 tid0 c1 c2)
       (WRITE: writing_event loc ts e0)
-      (FIND: IdentMap.find tid1 c1.(Configuration.threads) = Some (existT _ lang st0, lc0))
-      (THREAD_STEPS: Trace.steps tr (Thread.mk _ st0 lc0 c1.(Configuration.sc) c1.(Configuration.memory)) th1)
-      (PF: List.Forall (compose pf_event snd) tr)
+      (FIND: IdentMap.find tid1 c2.(Configuration.threads) = Some (existT _ lang st0, lc0))
+      (THREAD_STEPS: Trace.steps tr (Thread.mk _ st0 lc0 c2.(Configuration.sc) c2.(Configuration.memory)) th1)
+      (PF: List.Forall (compose (PF.pf_event L) snd) tr)
       (CONS: Local.promise_consistent th1.(Thread.local))
       (READ_STEP: Thread.step pf e1 th1 th2)
       (READ: reading_event loc ts e1)
       (LOC: L loc)
   .
 
-  Definition pf_multi_racefree_imm (c0: Configuration.t): Prop :=
+  Lemma step_racefree c0 c1 e tid
+        (RACEFREE: racefree c0)
+        (STEP: PFConfiguration.step L e tid c0 c1)
+    :
+      racefree c1.
+  Proof.
+    unfold racefree in *. i.
+    eapply RACEFREE. econs 2; eauto. econs; eauto.
+  Qed.
+
+  Lemma rtc_tau_machine_step_racefree c0 c1
+        (RACEFREE: racefree c0)
+        (STEP: rtc (PFConfiguration.tau_machine_step L) c0 c1)
+    :
+      racefree c1.
+  Proof.
+    ginduction STEP; eauto.
+    i. eapply IHSTEP. inv H. inv USTEP.
+    eapply step_racefree; eauto.
+  Qed.
+
+  Lemma steps_racefree es tid c0 c1
+        (RACEFREE: racefree c0)
+        (STEPS: PFConfiguration.steps L es tid c0 c1)
+    :
+      racefree c1.
+  Proof.
+    ginduction STEPS; eauto.
+    i. eapply IHSTEPS.
+    eapply step_racefree; eauto.
+  Qed.
+
+  Inductive multi_race (c0: Configuration.t): Prop :=
+  | multi_race_intro
+      c1
+      tid0 tid1 e0 e1
+      lang st0 lc0 th1 th2
+      e trs tr pf loc ts
+      (STEPS: PFConfiguration.step_trace L trs e tid0 c0 c1)
+      (TRACE: final_event_trace e0 trs)
+      (WRITE: writing_event loc ts e0)
+      (FIND: IdentMap.find tid1 c1.(Configuration.threads) = Some (existT _ lang st0, lc0))
+      (THREAD_STEPS: Trace.steps tr (Thread.mk _ st0 lc0 c1.(Configuration.sc) c1.(Configuration.memory)) th1)
+      (PF: List.Forall (compose (PF.pf_event L) snd) tr)
+      (CONS: Local.promise_consistent th1.(Thread.local))
+      (READ_STEP: Thread.step pf e1 th1 th2)
+      (READ: reading_event loc ts e1)
+      (LOC: L loc)
+  .
+
+  Definition multi_racefree_imm (c0: Configuration.t): Prop :=
     forall tid0 c1 trs0 tid1 c2 trs1
            loc ts lc1 te0 te1 e0 e1
            (LOC: L loc)
            (TID: tid0 <> tid1)
-           (CSTEP0: pf_step_trace trs0 e0 tid0 c0 c1)
+           (CSTEP0: PFConfiguration.step_trace L trs0 e0 tid0 c0 c1)
            (WRITE: writing_event loc ts te0)
            (TRACE0: final_event_trace te0 trs0)
-           (CSTEP1: pf_step_trace trs1 e1 tid1 c1 c2)
+           (CSTEP1: PFConfiguration.step_trace L trs1 e1 tid1 c1 c2)
            (READ: reading_event loc ts te1)
            (TRACE1: List.In (lc1, te1) trs1),
       False.
 
-  Definition pf_multi_racefree (c0: Configuration.t): Prop :=
+  Definition multi_racefree (c0: Configuration.t): Prop :=
     forall c1 trs
-           (CSTEPS: pf_steps_trace c0 c1 trs),
-      pf_multi_racefree_imm c1.
+           (CSTEPS: PFConfiguration.steps_trace L c0 c1 trs),
+      multi_racefree_imm c1.
 
-  Lemma multi_step_pf_multi_racefree c0 c1 tr e tid
-        (RACEFREE: pf_multi_racefree c0)
-        (STEP: pf_step_trace tr e tid c0 c1)
+  Lemma multi_step_multi_racefree c0 c1 tr e tid
+        (RACEFREE: multi_racefree c0)
+        (STEP: PFConfiguration.step_trace L tr e tid c0 c1)
     :
-      pf_multi_racefree c1.
+      multi_racefree c1.
   Proof.
-    unfold pf_multi_racefree in *. i.
+    unfold multi_racefree in *. i.
     eapply RACEFREE. econs 2; eauto.
   Qed.
 
-  Lemma multi_steps_pf_multi_racefree c0 c1 trs
-        (RACEFREE: pf_multi_racefree c0)
-        (STEPS: pf_steps_trace c0 c1 trs)
+  Lemma multi_steps_multi_racefree c0 c1 trs
+        (RACEFREE: multi_racefree c0)
+        (STEPS: PFConfiguration.steps_trace L c0 c1 trs)
     :
-      pf_multi_racefree c1.
+      multi_racefree c1.
   Proof.
     induction STEPS; auto. eapply IHSTEPS.
-    eapply multi_step_pf_multi_racefree; eauto.
+    eapply multi_step_multi_racefree; eauto.
   Qed.
 
-  Lemma reserving_trace_filter tr
-        (TRACE: reserving_trace tr)
-    :
-      List.filter ThreadEvent.is_normal_dec (List.map snd tr) = [].
-  Proof.
-    induction TRACE; eauto. ss. rewrite IHTRACE; eauto.
-    unfold ThreadEvent.is_normal, proj_sumbool in *. des_ifs.
-  Qed.
-
-  Lemma final_event_trace_filter tr e
-        (FINAL: final_event_trace e tr)
-        (NORMAL: ThreadEvent.is_normal e)
-    :
-      exists tr_hd,
-        (<<FILTER: List.filter ThreadEvent.is_normal_dec (List.map snd tr) = tr_hd ++ [e]>>).
-  Proof.
-    induction FINAL; eauto; i.
-    { exists []. ss. rewrite reserving_trace_filter; eauto.
-      unfold proj_sumbool. des_ifs. }
-    { des. ss. rewrite FILTER. des_ifs; eauto.
-      eexists. erewrite List.app_comm_cons. eauto.
-    }
-  Qed.
-
-  Lemma pf_racefree_multi_racefree_imm c
-        (RACEFREE: pf_racefree c)
+  Lemma racefree_multi_racefree_imm c
+        (RACEFREE: racefree c)
         (WF: Configuration.wf c)
-        (PF: pf_configuration c)
+        (PF: PF.pf_configuration L c)
     :
-      pf_multi_racefree_imm c.
+      multi_racefree_imm c.
   Proof.
-    ii. exploit pf_step_trace_future; try apply CSTEP0; eauto.  i. des.
+    ii. exploit PFConfiguration.step_trace_future; try apply CSTEP0; eauto.  i. des.
     exploit final_event_trace_filter; eauto.
     { unfold ThreadEvent.is_normal, ThreadEvent.is_reservation_event.
       inv WRITE; ss; ii; des; ss. } i. des.
-    eapply pf_step_trace_pf_steps in CSTEP0; eauto.
+    eapply PFConfiguration.step_trace_steps in CSTEP0; eauto.
     rewrite FILTER in *. des; cycle 1.
     { eapply List.app_eq_nil in NIL. des; ss. }
-    eapply pf_steps_split in STEPS. des. inv STEPS1. inv STEPS.
+    eapply PFConfiguration.steps_split in STEPS. des. inv STEPS1. inv STEPS.
     eapply List.in_split in TRACE1. des; subst.
-    dup CSTEP1. eapply pf_step_trace_pf_steps in CSTEP1; eauto.
+    dup CSTEP1. eapply PFConfiguration.step_trace_steps in CSTEP1; eauto.
     rewrite List.map_app in *.
     rewrite list_filter_app in *. ss. unfold proj_sumbool in *.
     des_ifs; cycle 1.
@@ -1099,10 +1110,10 @@ Proof.
       inv READ; ss; ii; des; ss. }
     des; cycle 1.
     { eapply List.app_eq_nil in NIL0. des; ss. }
-    eapply pf_steps_split in STEPS. des. inv STEPS2.
+    eapply PFConfiguration.steps_split in STEPS. des. inv STEPS2.
     eapply RACEFREE; try eassumption.
-    { eapply pf_steps_rtc_pf_all_step; eauto. }
-    { eapply silent_pf_steps_tau_pf_machine_steps; eauto.
+    { eapply PFConfiguration.steps_rtc_all_step; eauto. }
+    { eapply PFConfiguration.silent_steps_tau_machine_steps; eauto.
       clear - CSTEP0. inv CSTEP0.
       destruct (list_match_rev l2); des; subst.
       { eapply List.app_inj_tail in TR. des; clarify.
@@ -1121,42 +1132,42 @@ Proof.
     }
   Qed.
 
-  Lemma pf_racefree_multi_racefree c
-        (RACEFREE: pf_racefree c)
+  Lemma racefree_multi_racefree c
+        (RACEFREE: racefree c)
         (WF: Configuration.wf c)
-        (PF: pf_configuration c)
+        (PF: PF.pf_configuration L c)
     :
-      pf_multi_racefree c.
+      multi_racefree c.
   Proof.
-    unfold pf_multi_racefree. i.
+    unfold multi_racefree. i.
     ginduction CSTEPS; eauto.
-    { i. eapply pf_racefree_multi_racefree_imm; eauto. }
-    { i. exploit pf_step_trace_future; eauto.
+    { i. eapply racefree_multi_racefree_imm; eauto. }
+    { i. exploit PFConfiguration.step_trace_future; eauto.
       i. des. eapply IHCSTEPS; eauto.
-      eapply pf_step_trace_pf_steps in STEP; eauto. des.
-      { eapply steps_pf_racefree; eauto. }
-      { eapply reservation_only_step_pf_step in STEP0; eauto.
-        eapply step_pf_racefree; eauto. }
+      eapply PFConfiguration.step_trace_steps in STEP; eauto. des.
+      { eapply steps_racefree; eauto. }
+      { eapply PFConfiguration.reservation_only_step_step in STEP0; eauto.
+        eapply step_racefree; eauto. }
     }
   Qed.
 
-  Lemma pf_multi_race_pf_race c
-        (RACE: pf_multi_race c)
+  Lemma multi_race_race c
+        (RACE: multi_race c)
         (WF: Configuration.wf c)
-        (PF: pf_configuration c)
+        (PF: PF.pf_configuration L c)
     :
-      pf_racy_state c.
+      racy_state c.
   Proof.
     inv RACE.
-    exploit pf_step_trace_future; try apply STEPS; eauto. i. des.
+    exploit PFConfiguration.step_trace_future; try apply STEPS; eauto. i. des.
     exploit final_event_trace_filter; eauto.
     { ii. inv WRITE; eauto. } i. des.
-    dup STEPS. eapply pf_step_trace_pf_steps in STEPS; eauto.
+    dup STEPS. eapply PFConfiguration.step_trace_steps in STEPS; eauto.
     rewrite FILTER in *. des; cycle 1.
     { eapply List.app_eq_nil in NIL. des; ss. }
-    eapply pf_steps_split in STEPS1. des. inv STEPS3. inv STEPS.
+    eapply PFConfiguration.steps_split in STEPS1. des. inv STEPS3. inv STEPS.
     econs; cycle 1; eauto.
-    eapply silent_pf_steps_tau_pf_machine_steps; eauto.
+    eapply PFConfiguration.silent_steps_tau_machine_steps; eauto.
     assert (exists trs_hd trs_tl,
                (<<TRS: trs = trs_hd ++ [trs_tl]>>) /\
                (<<SILENT: List.Forall (fun the => ThreadEvent.get_machine_event (snd the) = MachineEvent.silent) trs_hd>>)).
@@ -1176,28 +1187,6 @@ Proof.
       eapply List.in_map_iff in H0. des. subst.
       eapply List.Forall_forall in SILENT; eauto.
     }
-  Qed.
-
-  Lemma pf_multi_step_behavior c
-        (WF: Configuration.wf c)
-        (PF: pf_configuration c)
-    :
-      behaviors pf_multi_step c <1= behaviors pf_machine_step c.
-  Proof.
-    i. induction PR.
-    - econs 1; eauto.
-    - exploit pf_multi_step_future; eauto. i. des.
-      eapply pf_multi_step_machine_step in STEP; eauto. des.
-      eapply rtc_tau_step_behavior; eauto.
-      inv STEP0; eauto. econs 2; eauto.
-    - exploit pf_multi_step_future; eauto. i. des.
-      eapply pf_multi_step_machine_step in STEP; eauto. des.
-      eapply rtc_tau_step_behavior; eauto.
-      inv STEP0; eauto. econs 3; eauto.
-    - exploit pf_multi_step_future; eauto. i. des.
-      eapply pf_multi_step_machine_step in STEP; eauto. des.
-      eapply rtc_tau_step_behavior; eauto.
-      inv STEP0; eauto. econs 4; eauto.
   Qed.
 
   Inductive racy_read (loc: Loc.t) (ts: Time.t):
@@ -1222,23 +1211,23 @@ Proof.
       racy_read loc ts lc (ThreadEvent.update loc ts to valr valw releasedr releasedw ordr ordw)
   .
 
-  Definition pf_multi_racefree_view (c0: Configuration.t): Prop :=
+  Definition multi_racefree_view (c0: Configuration.t): Prop :=
     forall c1 trs1 c2 trs2
       loc ts lc0 lc1 e0 e1
-      (CSTEPS1: pf_steps_trace c0 c1 trs1)
+      (CSTEPS1: PFConfiguration.steps_trace L c0 c1 trs1)
       (LOC: L loc)
       (TRACE1: List.In (lc0, e0) trs1)
       (WRITE: writing_event loc ts e0)
-      (CSTEPS2: pf_steps_trace c1 c2 trs2)
+      (CSTEPS2: PFConfiguration.steps_trace L c1 c2 trs2)
       (TRACE2: List.In (lc1, e1) trs2)
       (READ: racy_read loc ts lc1 e1),
       False.
 
-  Lemma multi_step_pf_multi_racefree_view c0 c1 tr e tid
-        (RACEFREE: pf_multi_racefree_view c0)
-        (STEP: pf_step_trace tr e tid c0 c1)
+  Lemma multi_step_multi_racefree_view c0 c1 tr e tid
+        (RACEFREE: multi_racefree_view c0)
+        (STEP: PFConfiguration.step_trace L tr e tid c0 c1)
     :
-      pf_multi_racefree_view c1.
+      multi_racefree_view c1.
   Proof.
     ii. eapply RACEFREE.
     { econs 2.
@@ -1253,68 +1242,70 @@ Proof.
     { eauto. }
   Qed.
 
-  Lemma multi_steps_pf_multi_racefree_view c0 c1 trs
-        (RACEFREE: pf_multi_racefree_view c0)
-        (STEPS: pf_steps_trace c0 c1 trs)
+  Lemma multi_steps_multi_racefree_view c0 c1 trs
+        (RACEFREE: multi_racefree_view c0)
+        (STEPS: PFConfiguration.steps_trace L c0 c1 trs)
     :
-      pf_multi_racefree_view c1.
+      multi_racefree_view c1.
   Proof.
     induction STEPS; auto. eapply IHSTEPS.
-    eapply multi_step_pf_multi_racefree_view; eauto.
+    eapply multi_step_multi_racefree_view; eauto.
   Qed.
 
-  Inductive pf_racy_read_step:
+  Inductive racy_read_step:
     forall (loc: Loc.t) (ts: Time.t)
            (e:ThreadEvent.t) (tid:Ident.t) (c1 c2:Configuration.t), Prop :=
-  | pf_racy_read_step_intro
+  | racy_read_step_intro
       loc ts e tid c1 lang st1 lc1 e2 e3 st4 lc4 sc4 memory4
       (TID: IdentMap.find tid c1.(Configuration.threads) = Some (existT _ lang st1, lc1))
       (CANCELS: rtc (@Thread.cancel_step _) (Thread.mk _ st1 lc1 c1.(Configuration.sc) c1.(Configuration.memory)) e2)
       (STEP: Thread.opt_step e e2 e3)
       (RESERVES: rtc (@Thread.reserve_step _) e3 (Thread.mk _ st4 lc4 sc4 memory4))
-      (CONSISTENT: e <> ThreadEvent.failure -> pf_consistent (Thread.mk _ st4 lc4 sc4 memory4))
-      (PF: pf_event e)
+      (CONSISTENT: e <> ThreadEvent.failure -> PF.pf_consistent L (Thread.mk _ st4 lc4 sc4 memory4))
+      (PF: PF.pf_event L e)
       (READ: racy_read loc ts e2.(Thread.local) e)
     :
-      pf_racy_read_step loc ts e tid c1 (Configuration.mk (IdentMap.add tid (existT _ _ st4, lc4) c1.(Configuration.threads)) sc4 memory4)
+      racy_read_step loc ts e tid c1 (Configuration.mk (IdentMap.add tid (existT _ _ st4, lc4) c1.(Configuration.threads)) sc4 memory4)
   .
-  Hint Constructors pf_racy_read_step.
+  Hint Constructors racy_read_step.
 
-  Inductive pf_racy_write_step:
+  Inductive racy_write_step:
     forall (loc: Loc.t) (ts: Time.t)
            (e:ThreadEvent.t) (tid:Ident.t) (c1 c2:Configuration.t), Prop :=
-  | pf_racy_write_step_intro
+  | racy_write_step_intro
       loc ts e tid c1 c2
-      (STEP: pf_step e tid c1 c2)
+      (STEP: PFConfiguration.step L e tid c1 c2)
       (WRITE: writing_event loc ts e)
     :
-      pf_racy_write_step loc ts e tid c1 c2
+      racy_write_step loc ts e tid c1 c2
   .
 
-  Definition pf_racefree_view (c0: Configuration.t): Prop :=
+  Definition racefree_view (c0: Configuration.t): Prop :=
     forall c1 c2 c3 c4 loc ts e0 e1 tid0 tid1
       (LOC: L loc)
-      (CSTEPS1: rtc pf_all_step c0 c1)
-      (WRITE: pf_racy_write_step loc ts e0 tid0 c1 c2)
-      (CSTEPS2: rtc pf_all_step c2 c3)
-      (READ: pf_racy_read_step loc ts e1 tid1 c3 c4),
+      (CSTEPS1: rtc (PFConfiguration.all_step L) c0 c1)
+      (WRITE: racy_write_step loc ts e0 tid0 c1 c2)
+      (CSTEPS2: rtc (PFConfiguration.all_step L) c2 c3)
+      (READ: racy_read_step loc ts e1 tid1 c3 c4),
       False.
 
-  Lemma step_pf_racefree_view c0 c1 e tid
-        (RACEFREE: pf_racefree_view c0)
-        (STEP: pf_step e tid c0 c1)
+  Lemma step_racefree_view c0 c1 e tid
+        (RACEFREE: racefree_view c0)
+        (STEP: PFConfiguration.step L e tid c0 c1)
     :
-      pf_racefree_view c1.
+      racefree_view c1.
   Proof.
     ii. eapply RACEFREE; cycle 2; eauto.
+    econs; eauto. econs; eauto.
   Qed.
 
-  Lemma steps_pf_racefree_view c0 c1
-        (RACEFREE: pf_racefree_view c0)
-        (STEPS: rtc pf_all_step c0 c1)
+  Lemma steps_racefree_view c0 c1
+        (RACEFREE: racefree_view c0)
+        (STEPS: rtc (PFConfiguration.all_step L) c0 c1)
     :
-      pf_racefree_view c1.
+      racefree_view c1.
   Proof.
     ii. eapply RACEFREE; cycle 2; eauto. etrans; eauto.
   Qed.
-End LOCALPF.
+End LOCALPFRACE.
+End PFRace.
